src/Reflection/Z/Bounds/Pipeline.v
@@ -1,0 +1,25 @@
+(** * Reflective Pipeline *)
+(** This file combines the various PHOAS modules in tactics,
+    culminating in a tactic [refine_reflectively], which solves a goal of the form
+<<
+cast_back_flat_const (?x args) = f (cast_back_flat_const args)
+ /\ Bounds.is_bounded_by ?bounds (?x args)
+>>
+while instantiating [?x] and [?bounds] with nicely-reduced constants.
+*)
+
+Ltac refine_reflectively := idtac.
+
+Require Import Crypto.Reflection.Syntax.
+Require Import Crypto.Reflection.Z.Syntax.
+Require Import Crypto.Reflection.Z.Bounds.Interpretation.
+Require Import Crypto.Reflection.Z.MapBounds.
+Require Import Crypto.Reflection.Z.MapBoundsInterp.
+Require Import Crypto.Reflection.Z.Syntax.Util.
+Require Import Crypto.Specific.GF25519.
+About cast_back_flat_const.
+
+Goal forall var src dst f' V V' f args, exists x bounds, @cast_back_flat_const var dst f' V (x args) = f (@cast_back_flat_const var src f' V' args) /\ Bounds.is_bounded_by bounds (x args).
+Proof.
+  intros; do 2 eexists.
+  refine (let k := MapBoundsPackagedCorrect in _).
