src/Specific/GF25519Reflective/Reified/Add.v
@@ -1,12 +1,21 @@
-Require Import Crypto.Specific.GF25519Reflective.CommonBinOp.
+Require Import Crypto.Specific.GF25519Reflective.Common.
 
 Definition raddZ_sig : rexpr_binop_sig add. Proof. reify_sig. Defined.
-Definition raddW := Eval vm_compute in rword_of_Z raddZ_sig.
-Lemma raddW_correct_and_bounded_gen : correct_and_bounded_genT raddW raddZ_sig.
-Proof. rexpr_correct. Qed.
-Definition radd_output_bounds := Eval vm_compute in compute_bounds raddW ExprBinOp_bounds.
+Definition raddZ : Expr _ := Eval vm_compute in proj1_sig raddZ_sig.
+Definition raddW_pkgo := Eval vm_compute in rexpr_select_word_sizes_option raddZ ExprBinOp_bounds.
+Definition raddW_pkg := Eval vm_compute in rexpr_select_word_sizes_postprocess1 raddW_pkgo.
+Definition raddT := get_output_type raddW_pkg.
+Definition raddW' : Expr _ := Eval vm_compute in get_output_expr raddW_pkg.
+Definition raddW : Expr raddT := Eval cbv [raddW'] in rexpr_select_word_sizes_postprocess2 raddW'.
+Definition radd_output_bounds := Eval vm_compute in get_bounds raddW_pkg.
+Definition raddZ_Wf : rexpr_wfT raddZ. Proof. prove_rexpr_wfT. Qed.
+Local Obligation Tactic := rexpr_correct_and_bounded_obligation_tac.
+Program Definition raddZ_correct_and_bounded_tight
+  : rexpr_correct_and_boundedT raddZ raddW ExprBinOp_bounds radd_output_bounds
+  := rexpr_correct_and_bounded raddZ raddW ExprBinOp_bounds radd_output_bounds raddZ_Wf.
 
 Local Open Scope string_scope.
-Compute ("Add", compute_bounds_for_display raddW ExprBinOp_bounds).
-Compute ("Add overflows? ", sanity_compute raddW ExprBinOp_bounds).
-Compute ("Add overflows (error if it does)? ", sanity_check raddW ExprBinOp_bounds).
+Compute ("Add", compute_bounds_for_display raddW_pkg).
+(* We use [compute] rather than [vm_compute] so as to not eta-expand functions, so we get pretty display *)
+Eval compute in ("Add overflows? ", sanity_compute raddW_pkg).
+Compute ("Add overflows (error if it does)? ", sanity_check raddW_pkg).
