src/Specific/GF25519Reflective/Reified/CarryAdd.v
@@ -1,17 +1,21 @@
-Require Import Crypto.Specific.GF25519Reflective.CommonBinOp.
+Require Import Crypto.Specific.GF25519Reflective.Common.
 
 Definition rcarry_addZ_sig : rexpr_binop_sig carry_add. Proof. reify_sig. Defined.
-Definition rcarry_addW := Eval vm_compute in rword_of_Z rcarry_addZ_sig.
-Lemma rcarry_addW_correct_and_bounded_gen : correct_and_bounded_genT rcarry_addW rcarry_addZ_sig.
-Proof. rexpr_correct. Qed.
-Definition rcarry_add_output_bounds := Eval vm_compute in compute_bounds rcarry_addW ExprBinOp_bounds.
-Local Obligation Tactic := intros; vm_compute; constructor.
-Program Definition rcarry_addW_correct_and_bounded
-  := ExprBinOp_correct_and_bounded
-       rcarry_addW carry_add rcarry_addZ_sig rcarry_addW_correct_and_bounded_gen
-       _ _.
+Definition rcarry_addZ : Expr _ := Eval vm_compute in proj1_sig rcarry_addZ_sig.
+Definition rcarry_addW_pkgo := Eval vm_compute in rexpr_select_word_sizes_option rcarry_addZ ExprBinOp_bounds.
+Definition rcarry_addW_pkg := Eval vm_compute in rexpr_select_word_sizes_postprocess1 rcarry_addW_pkgo.
+Definition rcarry_addT := get_output_type rcarry_addW_pkg.
+Definition rcarry_addW' : Expr _ := Eval vm_compute in get_output_expr rcarry_addW_pkg.
+Definition rcarry_addW : Expr rcarry_addT := Eval cbv [rcarry_addW'] in rexpr_select_word_sizes_postprocess2 rcarry_addW'.
+Definition rcarry_add_output_bounds := Eval vm_compute in get_bounds rcarry_addW_pkg.
+Definition rcarry_addZ_Wf : rexpr_wfT rcarry_addZ. Proof. prove_rexpr_wfT. Qed.
+Local Obligation Tactic := rexpr_correct_and_bounded_obligation_tac.
+Program Definition rcarry_addZ_correct_and_bounded_tight
+  : rexpr_correct_and_boundedT rcarry_addZ rcarry_addW ExprBinOp_bounds rcarry_add_output_bounds
+  := rexpr_correct_and_bounded rcarry_addZ rcarry_addW ExprBinOp_bounds rcarry_add_output_bounds rcarry_addZ_Wf.
 
 Local Open Scope string_scope.
-Compute ("Carry_Add", compute_bounds_for_display rcarry_addW ExprBinOp_bounds).
-Compute ("Carry_Add overflows? ", sanity_compute rcarry_addW ExprBinOp_bounds).
-Compute ("Carry_Add overflows (error if it does)? ", sanity_check rcarry_addW ExprBinOp_bounds).
+Compute ("Carry_Add", compute_bounds_for_display rcarry_addW_pkg).
+(* We use [compute] rather than [vm_compute] so as to not eta-expand functions, so we get pretty display *)
+Eval compute in ("Carry_Add overflows? ", sanity_compute rcarry_addW_pkg).
+Compute ("Carry_Add overflows (error if it does)? ", sanity_check rcarry_addW_pkg).
