src/Specific/GF25519Reflective/Reified/CarryOpp.v
@@ -1,17 +1,21 @@
-Require Import Crypto.Specific.GF25519Reflective.CommonUnOp.
+Require Import Crypto.Specific.GF25519Reflective.Common.
 
 Definition rcarry_oppZ_sig : rexpr_unop_sig carry_opp. Proof. reify_sig. Defined.
-Definition rcarry_oppW := Eval vm_compute in rword_of_Z rcarry_oppZ_sig.
-Lemma rcarry_oppW_correct_and_bounded_gen : correct_and_bounded_genT rcarry_oppW rcarry_oppZ_sig.
-Proof. rexpr_correct. Qed.
-Definition rcarry_opp_output_bounds := Eval vm_compute in compute_bounds rcarry_oppW ExprUnOp_bounds.
-Local Obligation Tactic := intros; vm_compute; constructor.
-Program Definition rcarry_oppW_correct_and_bounded
-  := ExprUnOp_correct_and_bounded
-       rcarry_oppW carry_opp rcarry_oppZ_sig rcarry_oppW_correct_and_bounded_gen
-       _ _.
+Definition rcarry_oppZ : Expr _ := Eval vm_compute in proj1_sig rcarry_oppZ_sig.
+Definition rcarry_oppW_pkgo := Eval vm_compute in rexpr_select_word_sizes_option rcarry_oppZ ExprUnOp_bounds.
+Definition rcarry_oppW_pkg := Eval vm_compute in rexpr_select_word_sizes_postprocess1 rcarry_oppW_pkgo.
+Definition rcarry_oppT := get_output_type rcarry_oppW_pkg.
+Definition rcarry_oppW' : Expr _ := Eval vm_compute in get_output_expr rcarry_oppW_pkg.
+Definition rcarry_oppW : Expr rcarry_oppT := Eval cbv [rcarry_oppW'] in rexpr_select_word_sizes_postprocess2 rcarry_oppW'.
+Definition rcarry_opp_output_bounds := Eval vm_compute in get_bounds rcarry_oppW_pkg.
+Definition rcarry_oppZ_Wf : rexpr_wfT rcarry_oppZ. Proof. prove_rexpr_wfT. Qed.
+Local Obligation Tactic := rexpr_correct_and_bounded_obligation_tac.
+Program Definition rcarry_oppZ_correct_and_bounded_tight
+  : rexpr_correct_and_boundedT rcarry_oppZ rcarry_oppW ExprUnOp_bounds rcarry_opp_output_bounds
+  := rexpr_correct_and_bounded rcarry_oppZ rcarry_oppW ExprUnOp_bounds rcarry_opp_output_bounds rcarry_oppZ_Wf.
 
 Local Open Scope string_scope.
-Compute ("Carry_Opp", compute_bounds_for_display rcarry_oppW ExprUnOp_bounds).
-Compute ("Carry_Opp overflows? ", sanity_compute rcarry_oppW ExprUnOp_bounds).
-Compute ("Carry_Opp overflows (error if it does)? ", sanity_check rcarry_oppW ExprUnOp_bounds).
+Compute ("Carry_Opp", compute_bounds_for_display rcarry_oppW_pkg).
+(* We use [compute] rather than [vm_compute] so as to not eta-expand functions, so we get pretty display *)
+Eval compute in ("Carry_Opp overflows? ", sanity_compute rcarry_oppW_pkg).
+Compute ("Carry_Opp overflows (error if it does)? ", sanity_check rcarry_oppW_pkg).
