src/Specific/GF25519Reflective/Reified/CarrySub.v
@@ -1,17 +1,21 @@
-Require Import Crypto.Specific.GF25519Reflective.CommonBinOp.
+Require Import Crypto.Specific.GF25519Reflective.Common.
 
 Definition rcarry_subZ_sig : rexpr_binop_sig carry_sub. Proof. reify_sig. Defined.
-Definition rcarry_subW := Eval vm_compute in rword_of_Z rcarry_subZ_sig.
-Lemma rcarry_subW_correct_and_bounded_gen : correct_and_bounded_genT rcarry_subW rcarry_subZ_sig.
-Proof. rexpr_correct. Qed.
-Definition rcarry_sub_output_bounds := Eval vm_compute in compute_bounds rcarry_subW ExprBinOp_bounds.
-Local Obligation Tactic := intros; vm_compute; constructor.
-Program Definition rcarry_subW_correct_and_bounded
-  := ExprBinOp_correct_and_bounded
-       rcarry_subW carry_sub rcarry_subZ_sig rcarry_subW_correct_and_bounded_gen
-       _ _.
+Definition rcarry_subZ : Expr _ := Eval vm_compute in proj1_sig rcarry_subZ_sig.
+Definition rcarry_subW_pkgo := Eval vm_compute in rexpr_select_word_sizes_option rcarry_subZ ExprBinOp_bounds.
+Definition rcarry_subW_pkg := Eval vm_compute in rexpr_select_word_sizes_postprocess1 rcarry_subW_pkgo.
+Definition rcarry_subT := get_output_type rcarry_subW_pkg.
+Definition rcarry_subW' : Expr _ := Eval vm_compute in get_output_expr rcarry_subW_pkg.
+Definition rcarry_subW : Expr rcarry_subT := Eval cbv [rcarry_subW'] in rexpr_select_word_sizes_postprocess2 rcarry_subW'.
+Definition rcarry_sub_output_bounds := Eval vm_compute in get_bounds rcarry_subW_pkg.
+Definition rcarry_subZ_Wf : rexpr_wfT rcarry_subZ. Proof. prove_rexpr_wfT. Qed.
+Local Obligation Tactic := rexpr_correct_and_bounded_obligation_tac.
+Program Definition rcarry_subZ_correct_and_bounded_tight
+  : rexpr_correct_and_boundedT rcarry_subZ rcarry_subW ExprBinOp_bounds rcarry_sub_output_bounds
+  := rexpr_correct_and_bounded rcarry_subZ rcarry_subW ExprBinOp_bounds rcarry_sub_output_bounds rcarry_subZ_Wf.
 
 Local Open Scope string_scope.
-Compute ("Carry_Sub", compute_bounds_for_display rcarry_subW ExprBinOp_bounds).
-Compute ("Carry_Sub overflows? ", sanity_compute rcarry_subW ExprBinOp_bounds).
-Compute ("Carry_Sub overflows (error if it does)? ", sanity_check rcarry_subW ExprBinOp_bounds).
+Compute ("Carry_Sub", compute_bounds_for_display rcarry_subW_pkg).
+(* We use [compute] rather than [vm_compute] so as to not eta-expand functions, so we get pretty display *)
+Eval compute in ("Carry_Sub overflows? ", sanity_compute rcarry_subW_pkg).
+Compute ("Carry_Sub overflows (error if it does)? ", sanity_check rcarry_subW_pkg).
