src/Specific/GF25519Reflective/Reified/Mul.v
@@ -1,17 +1,21 @@
-Require Import Crypto.Specific.GF25519Reflective.CommonBinOp.
+Require Import Crypto.Specific.GF25519Reflective.Common.
 
 Definition rmulZ_sig : rexpr_binop_sig mul. Proof. reify_sig. Defined.
-Definition rmulW := Eval vm_compute in rword_of_Z rmulZ_sig.
-Lemma rmulW_correct_and_bounded_gen : correct_and_bounded_genT rmulW rmulZ_sig.
-Proof. rexpr_correct. Qed.
-Definition rmul_output_bounds := Eval vm_compute in compute_bounds rmulW ExprBinOp_bounds.
-Local Obligation Tactic := intros; vm_compute; constructor.
-Program Definition rmulW_correct_and_bounded
-  := ExprBinOp_correct_and_bounded
-       rmulW mul rmulZ_sig rmulW_correct_and_bounded_gen
-       _ _.
+Definition rmulZ : Expr _ := Eval vm_compute in proj1_sig rmulZ_sig.
+Definition rmulW_pkgo := Eval vm_compute in rexpr_select_word_sizes_option rmulZ ExprBinOp_bounds.
+Definition rmulW_pkg := Eval vm_compute in rexpr_select_word_sizes_postprocess1 rmulW_pkgo.
+Definition rmulT := get_output_type rmulW_pkg.
+Definition rmulW' : Expr _ := Eval vm_compute in get_output_expr rmulW_pkg.
+Definition rmulW : Expr rmulT := Eval cbv [rmulW'] in rexpr_select_word_sizes_postprocess2 rmulW'.
+Definition rmul_output_bounds := Eval vm_compute in get_bounds rmulW_pkg.
+Definition rmulZ_Wf : rexpr_wfT rmulZ. Proof. prove_rexpr_wfT. Qed.
+Local Obligation Tactic := rexpr_correct_and_bounded_obligation_tac.
+Program Definition rmulZ_correct_and_bounded_tight
+  : rexpr_correct_and_boundedT rmulZ rmulW ExprBinOp_bounds rmul_output_bounds
+  := rexpr_correct_and_bounded rmulZ rmulW ExprBinOp_bounds rmul_output_bounds rmulZ_Wf.
 
 Local Open Scope string_scope.
-Compute ("Mul", compute_bounds_for_display rmulW ExprBinOp_bounds).
-Compute ("Mul overflows? ", sanity_compute rmulW ExprBinOp_bounds).
-Compute ("Mul overflows (error if it does)? ", sanity_check rmulW ExprBinOp_bounds).
+Compute ("Mul", compute_bounds_for_display rmulW_pkg).
+(* We use [compute] rather than [vm_compute] so as to not eta-expand functions, so we get pretty display *)
+Eval compute in ("Mul overflows? ", sanity_compute rmulW_pkg).
+Compute ("Mul overflows (error if it does)? ", sanity_check rmulW_pkg).
