src/Specific/GF25519Reflective/Reified/PreFreeze.v
@@ -1,17 +1,21 @@
-Require Import Crypto.Specific.GF25519Reflective.CommonUnOp.
+Require Import Crypto.Specific.GF25519Reflective.Common.
 
 Definition rprefreezeZ_sig : rexpr_unop_sig prefreeze. Proof. reify_sig. Defined.
-Definition rprefreezeW := Eval vm_compute in rword_of_Z rprefreezeZ_sig.
-Lemma rprefreezeW_correct_and_bounded_gen : correct_and_bounded_genT rprefreezeW rprefreezeZ_sig.
-Proof. rexpr_correct. Qed.
-Definition rprefreeze_output_bounds := Eval vm_compute in compute_bounds rprefreezeW ExprUnOp_bounds.
-Local Obligation Tactic := intros; vm_compute; constructor.
-Program Definition rprefreezeW_correct_and_bounded
-  := ExprUnOp_correct_and_bounded
-       rprefreezeW prefreeze rprefreezeZ_sig rprefreezeW_correct_and_bounded_gen
-       _ _.
+Definition rprefreezeZ : Expr _ := Eval vm_compute in proj1_sig rprefreezeZ_sig.
+Definition rprefreezeW_pkgo := Eval vm_compute in rexpr_select_word_sizes_option rprefreezeZ ExprUnOp_bounds.
+Definition rprefreezeW_pkg := Eval vm_compute in rexpr_select_word_sizes_postprocess1 rprefreezeW_pkgo.
+Definition rprefreezeT := get_output_type rprefreezeW_pkg.
+Definition rprefreezeW' : Expr _ := Eval vm_compute in get_output_expr rprefreezeW_pkg.
+Definition rprefreezeW : Expr rprefreezeT := Eval cbv [rprefreezeW'] in rexpr_select_word_sizes_postprocess2 rprefreezeW'.
+Definition rprefreeze_output_bounds := Eval vm_compute in get_bounds rprefreezeW_pkg.
+Definition rprefreezeZ_Wf : rexpr_wfT rprefreezeZ. Proof. prove_rexpr_wfT. Qed.
+Local Obligation Tactic := rexpr_correct_and_bounded_obligation_tac.
+Program Definition rprefreezeZ_correct_and_bounded_tight
+  : rexpr_correct_and_boundedT rprefreezeZ rprefreezeW ExprUnOp_bounds rprefreeze_output_bounds
+  := rexpr_correct_and_bounded rprefreezeZ rprefreezeW ExprUnOp_bounds rprefreeze_output_bounds rprefreezeZ_Wf.
 
 Local Open Scope string_scope.
-Compute ("PreFreeze", compute_bounds_for_display rprefreezeW ExprUnOp_bounds).
-Compute ("PreFreeze overflows? ", sanity_compute rprefreezeW ExprUnOp_bounds).
-Compute ("PreFreeze overflows (error if it does)? ", sanity_check rprefreezeW ExprUnOp_bounds).
+Compute ("PreFreeze", compute_bounds_for_display rprefreezeW_pkg).
+(* We use [compute] rather than [vm_compute] so as to not eta-expand functions, so we get pretty display *)
+Eval compute in ("PreFreeze overflows? ", sanity_compute rprefreezeW_pkg).
+Compute ("PreFreeze overflows (error if it does)? ", sanity_check rprefreezeW_pkg).
