src/Specific/GF25519Reflective/Reified/Unpack.v
@@ -1,17 +1,21 @@
-Require Import Crypto.Specific.GF25519Reflective.CommonUnOpWireToFE.
+Require Import Crypto.Specific.GF25519Reflective.Common.
 
 Definition runpackZ_sig : rexpr_unop_WireToFE_sig unpack. Proof. reify_sig. Defined.
-Definition runpackW := Eval vm_compute in rword_of_Z runpackZ_sig.
-Lemma runpackW_correct_and_bounded_gen : correct_and_bounded_genT runpackW runpackZ_sig.
-Proof. rexpr_correct. Qed.
-Definition runpack_output_bounds := Eval vm_compute in compute_bounds runpackW ExprUnOpWireToFE_bounds.
-Local Obligation Tactic := intros; vm_compute; constructor.
-Program Definition runpackW_correct_and_bounded
-  := ExprUnOpWireToFE_correct_and_bounded
-       runpackW unpack runpackZ_sig runpackW_correct_and_bounded_gen
-       _ _.
+Definition runpackZ : Expr _ := Eval vm_compute in proj1_sig runpackZ_sig.
+Definition runpackW_pkgo := Eval vm_compute in rexpr_select_word_sizes_option runpackZ ExprUnOpWireToFE_bounds.
+Definition runpackW_pkg := Eval vm_compute in rexpr_select_word_sizes_postprocess1 runpackW_pkgo.
+Definition runpackT := get_output_type runpackW_pkg.
+Definition runpackW' : Expr _ := Eval vm_compute in get_output_expr runpackW_pkg.
+Definition runpackW : Expr runpackT := Eval cbv [runpackW'] in rexpr_select_word_sizes_postprocess2 runpackW'.
+Definition runpack_output_bounds := Eval vm_compute in get_bounds runpackW_pkg.
+Definition runpackZ_Wf : rexpr_wfT runpackZ. Proof. prove_rexpr_wfT. Qed.
+Local Obligation Tactic := rexpr_correct_and_bounded_obligation_tac.
+Program Definition runpackZ_correct_and_bounded_tight
+  : rexpr_correct_and_boundedT runpackZ runpackW ExprUnOpWireToFE_bounds runpack_output_bounds
+  := rexpr_correct_and_bounded runpackZ runpackW ExprUnOpWireToFE_bounds runpack_output_bounds runpackZ_Wf.
 
 Local Open Scope string_scope.
-Compute ("Unpack", compute_bounds_for_display runpackW ExprUnOpWireToFE_bounds).
-Compute ("Unpack overflows? ", sanity_compute runpackW ExprUnOpWireToFE_bounds).
-Compute ("Unpack overflows (error if it does)? ", sanity_check runpackW ExprUnOpWireToFE_bounds).
+Compute ("Unpack", compute_bounds_for_display runpackW_pkg).
+(* We use [compute] rather than [vm_compute] so as to not eta-expand functions, so we get pretty display *)
+Eval compute in ("Unpack overflows? ", sanity_compute runpackW_pkg).
+Compute ("Unpack overflows (error if it does)? ", sanity_check runpackW_pkg).
