src/SpecificGen/GF2519_32Reflective/Reified/Add.v
@@ -1,12 +1,16 @@
-Require Import Crypto.SpecificGen.GF2519_32Reflective.CommonBinOp.
+Require Import Crypto.SpecificGen.GF2519_32Reflective.Common.
 
 Definition raddZ_sig : rexpr_binop_sig add. Proof. reify_sig. Defined.
-Definition raddW := Eval vm_compute in rword_of_Z raddZ_sig.
-Lemma raddW_correct_and_bounded_gen : correct_and_bounded_genT raddW raddZ_sig.
-Proof. rexpr_correct. Qed.
-Definition radd_output_bounds := Eval vm_compute in compute_bounds raddW ExprBinOp_bounds.
+Definition raddZ : Syntax.Expr _ _ _ := Eval vm_compute in proj1_sig raddZ_sig.
+Definition raddW : Syntax.Expr _ _ _ := Eval vm_compute in rexpr_select_word_sizes raddZ ExprBinOp_bounds.
+Definition raddZ_Wf : rexpr_wfT raddZ. Proof. prove_rexpr_wfT. Qed.
+Definition radd_output_bounds
+  := Eval vm_compute in compute_bounds raddZ ExprBinOp_bounds.
+Local Obligation Tactic := intros; vm_compute; constructor.
+Program Definition raddZ_correct_and_bounded
+  := rexpr_correct_and_bounded raddZ raddZ_Wf ExprBinOp_bounds.
 
 Local Open Scope string_scope.
-Compute ("Add", compute_bounds_for_display raddW ExprBinOp_bounds).
-Compute ("Add overflows? ", sanity_compute raddW ExprBinOp_bounds).
-Compute ("Add overflows (error if it does)? ", sanity_check raddW ExprBinOp_bounds).
+Compute ("Add", compute_bounds_for_display raddZ ExprBinOp_bounds).
+Compute ("Add overflows? ", sanity_compute raddZ ExprBinOp_bounds).
+Compute ("Add overflows (error if it does)? ", sanity_check raddZ ExprBinOp_bounds).
